Saving a lot of cleanup work up to the point of cvm verif, proof them become SUPER hard

src/Cvm_Monad.v
@@ -92,16 +92,30 @@ Definition hoist_result {A : Type} (r : ResultT A string) : CVM A :=
   | errC e => err_failm (dispatch_error (Runtime e))
   end.
 
+Definition get_asp_type (a : ASP_ID) : CVM EvSig :=
+  sc <- get_config ;;
+  let G := session_context sc in
+  match (map_get a (asp_types G)) with
+  | None => err_failm (dispatch_error (Runtime err_str_asp_no_type_sig))
+  | Some ev => err_ret ev
+  end.
+
+Definition get_asp_dual (a : ASP_ID) : CVM ASP_ID :=
+  sc <- get_config ;;
+  let G := session_context sc in
+  match (map_get a (asp_comps G)) with
+  | None => err_failm (dispatch_error (Runtime err_str_asp_no_compat_appr_asp))
+  | Some appr_asp_id => err_ret appr_asp_id
+  end.
+
 (* Helper function that builds a new internal EvidenceT bundle based on 
    the EvidenceT extension parameter of an ASP term. *)
 Definition bundle_asp (p:Plc) (rwev : RawEv) 
     (cur_ev : Evidence) (ps:ASP_PARAMS) : CVM Evidence :=
-  sc <- get_config ;;
-  let G := session_context sc in
   let '(asp_paramsC asp_id args targ_plc targ) := ps in
-  match (map_get asp_id (asp_types G)) with
-  | None => err_failm (dispatch_error (Runtime err_str_asp_no_type_sig))
-  | Some (ev_arrow fwd in_sig (OutN n)) =>
+  '(ev_arrow fwd in_sig out_sig) <- get_asp_type asp_id ;;
+  match out_sig with
+  | (OutN n) =>
     if (eqb (length rwev) n)
     then 
       match fwd with
@@ -114,7 +128,7 @@ attestation and bundling side of the CVM. Wraps main distinction lies in the
 fact that its is a GUARANTEE, that the dual appraisal ASP is actually an
 inverse, thus allowing WRAPPED evidence to be recovered via appraisal *)
       | WRAP => err_ret (evc rwev (asp_evt p ps (get_et cur_ev)))
-      | UNWRAP => err_failm (dispatch_error (Runtime "UNWRAP ASPs must have OutUnwrap"))
+      | UNWRAP => err_failm (dispatch_error (Runtime err_str_unwrap_must_have_outwrap))
 (* The semantics for an "EXTEND" asp are it APPENDS all incoming evidence to the
 current CVM evidence bundle *)
       | EXTEND =>
@@ -123,19 +137,21 @@ current CVM evidence bundle *)
         end
       end
     else err_failm (dispatch_error (Runtime errStr_raw_EvidenceT_too_long))
-  | Some (ev_arrow fwd in_sig OutUnwrap) => 
+  | OutUnwrap =>
     match fwd with
-    | WRAP => err_failm (dispatch_error (Runtime "WRAP ASPs cannot have OutUnwrap"))
-    | REPLACE => err_failm (dispatch_error (Runtime "REPLACE ASPs cannot have OutUnwrap"))
-    | EXTEND => err_failm (dispatch_error (Runtime "EXTEND ASPs cannot have OutUnwrap"))
+    | WRAP => err_failm (dispatch_error (Runtime err_str_only_unwrap_can_be_outwrap))
+    | REPLACE => err_failm (dispatch_error (Runtime err_str_only_unwrap_can_be_outwrap))
+    | EXTEND => err_failm (dispatch_error (Runtime err_str_only_unwrap_can_be_outwrap))
     | UNWRAP => 
+      sc <- get_config ;;
+      let G := (session_context sc) in
       let '(evc bits et) := cur_ev in
       r <- hoist_result (get_asp_under G et) ;;
       match r with
       | asp_evt p' (asp_paramsC wrap_id _ _ _) et' =>
-        match (map_get wrap_id (asp_types G)) with
-        | None => err_failm (dispatch_error (Runtime err_str_asp_no_type_sig))
-        | Some (ev_arrow WRAP _ _) =>
+        '(ev_arrow fwd _ _) <- get_asp_type wrap_id ;;
+        match fwd with
+        | WRAP =>
           (* we are an UNWRAP or a WRAP, so new size is the sizer of et' *)
           match et_size G et' with
           | errC e => err_failm (dispatch_error (Runtime e))
@@ -143,11 +159,11 @@ current CVM evidence bundle *)
             if (eqb (length rwev) et'_size)
             then (* we are the right inverse size! *)
               err_ret (evc rwev (asp_evt p ps et))
-            else err_failm (dispatch_error (Runtime "UNWRAP of a WRAP ASP must have the same size of the WRAPed evidence"))
+            else err_failm (dispatch_error (Runtime err_str_unwrap_of_wrap_same_size))
           end
-        | Some (ev_arrow _ _ _) => err_failm (dispatch_error (Runtime "UNWRAP ASPs must be applied to a WRAP ASP"))
+        | _ => err_failm (dispatch_error (Runtime err_str_unwrap_only_wrap))
         end
-      | _ => err_failm (dispatch_error (Runtime "UNWRAP ASPs must be applied to a WRAP ASP"))
+      | _ => err_failm (dispatch_error (Runtime err_str_unwrap_only_wrap))
       end
     end
   end.
@@ -185,75 +201,6 @@ Fixpoint peel_n_rawev (n : nat) (ls : RawEv) : ResultT (RawEv * RawEv) string :=
     end
   end.
 
-(*
-
-Open Scope string_scope.
-
-Definition split_evidence (G : GlobalContext) (et1 et2 : EvidenceT) :
-    EvidenceT -> ResultT (Evidence * Evidence) string :=
-  fix split_evidence' (e : Evidence) : ResultT (Evidence * Evidence) string :=
-  let '(evc bits et) := e in
-  match et with
-  | mt_evt => errC "Cannot split null evidence!"
-  | nonce_evt _ => errC "Cannot split nonce evidence!"
-  | asp_evt _ _ _ => errC "Cannot split ASP evidence!"
-  | left_evt e' => r <- apply_to_left_evt G split_evidence' e' ;; r
-  | right_evt e' => r <- apply_to_right_evt G split_evidence' e' ;; r
-  | split_evt et1' et2' =>
-    if (eqb et1 et1')
-    then 
-      if (eqb et2 et2')
-      then 
-        et1_size <- et_size G et1 ;;
-        et2_size <- et_size G et2 ;;
-        '(l_ev, rest) <- (peel_n_rawev et1_size bits) ;;
-        '(r_ev, rest') <- (peel_n_rawev et2_size rest) ;;
-        match rest' with
-        | [] => resultC (evc l_ev et1, evc r_ev et2)
-        | _ => errC "Evidence splitting failed: Rest of evidence not empty"
-        end
-      else errC "Evidence splitting failed: et2 does not match"
-    else errC "Evidence splitting failed: et1 does not match"
-  end.
-
-Definition split_evidence (e : Evidence) (et1 et2 : EvidenceT) 
-    : CVM (Evidence * Evidence) :=
-  sc <- get_config ;;
-  let G := (session_context sc) in
-  match (get_et e) with
-  | mt_evt => err_failm (dispatch_error (Runtime "Cannot split null evidence!"))
-  | nonce_evt _ => err_failm (dispatch_error (Runtime "Cannot split nonce evidence!"))
-  | asp_evt _ _ _ => err_failm (dispatch_error (Runtime "Cannot split ASP evidence!"))
-  | left_evt e' => 
-    apply_to_left_evt 
-    err_failm (dispatch_error (Runtime "Cannot split left_evt evidence!"))
-  | right_evt _ => err_failm (dispatch_error (Runtime "Cannot split right_evt evidence!"))
-  | split_evt et1' et2' =>
-    if (eqb et1 et1')
-    then 
-      if (eqb et2 et2')
-      then 
-        let r := get_bits e in
-        match et_size G et1 with
-        | errC e => err_failm (dispatch_error (Runtime e))
-        | resultC et1_size => 
-          match et_size G et2 with
-          | errC e => err_failm (dispatch_error (Runtime e))
-          | resultC et2_size =>
-            '(l_ev, rest) <- (hoist_result (peel_n_rawev et1_size r)) ;;
-            '(r_ev, rest') <- (hoist_result (peel_n_rawev et2_size rest)) ;;
-            match rest' with
-            | [] => err_ret (evc l_ev et1, evc r_ev et2)
-            | _ => err_failm (dispatch_error (Runtime "Evidence splitting failed: Rest of evidence not empty"))
-            end
-          end
-        end
-      else err_failm (dispatch_error (Runtime "Evidence splitting failed: et2 does not match"))
-    else err_failm (dispatch_error (Runtime "Evidence splitting failed: et1 does not match"))
-  end.
-*)
-
-Definition mt_test := mt_evt.
 (* Simulates invoking an arbitrary ASP.  Tags the event, builds and returns 
    the new EvidenceT bundle. *)
 
@@ -265,86 +212,58 @@ Fixpoint invoke_APPR' (r : RawEv) (et : EvidenceT) (out_evt : EvidenceT) {struct
   | nonce_evt n' => invoke_ASP (evc r out_evt) check_nonce_params
   | asp_evt p' par et' =>
     let '(asp_paramsC asp_id args targ_plc targ) := par in
-    match (map_get asp_id (asp_comps G)) with
-    | None => err_failm (dispatch_error (Runtime err_str_asp_no_compat_appr_asp))
-    | Some appr_asp_id =>
-      let dual_par := asp_paramsC appr_asp_id args targ_plc targ in
-      match (map_get asp_id (asp_types G)) with
-      | None => err_failm (dispatch_error (Runtime err_str_asp_no_type_sig))
-      | Some (ev_arrow fwd in_sig out_sig) =>
-        match fwd with
-        | REPLACE => (* Only do the dual ASP *)
-          invoke_ASP (evc r out_evt) dual_par
-        | WRAP =>
-          (* first do the dual ASP to unwrap *)
-          '(evc r'' et'') <- invoke_ASP (evc r out_evt) dual_par ;;
-          (* Check that the "UNWRAP" occured properly *)
-          match et_size G et'' with
-          | errC e => err_failm (dispatch_error (Runtime e))
-          | resultC n' => 
-            match et_size G et' with
-            | errC e => err_failm (dispatch_error (Runtime e))
-            | resultC n'' =>
-              if (eqb n' n'')
-              then (* The "UNWRAP" worked *)
-                (* so do the recursive call *)
-                invoke_APPR' r'' et' (asp_evt (session_plc sc) dual_par out_evt)
-              else err_failm (dispatch_error (Runtime "Appraisal for WRAP ASP failed. Size of input to wrap is not same as output of UNWRAP"))
-            end
-          end
-        | UNWRAP =>
-          (* to appraise an UNWRAP is to appraise whatever is below 
-          the UNWRAP and WRAP *)
-          match out_sig with
-          | OutN _ => err_failm (dispatch_error (Runtime "UNWRAP ASPs must have OutUnwrap"))
-          | OutUnwrap =>
-            e <- hoist_result (
-              apply_to_asp_under_wrap G asp_id (fun e => invoke_APPR' r e out_evt) et'
-            ) ;;
-            e
-            (* 
-            (* get the ASP under et' (NOTE: It better be a WRAP) *)
-            und <- hoist_result (get_asp_under G et') ;;
-            match und with
-            | asp_evt p' (asp_paramsC wrap_id _ _ _) et' =>
-              match (map_get wrap_id (asp_types G)) with
-              | None => err_failm (dispatch_error (Runtime err_str_asp_no_type_sig))
-              | Some (ev_arrow WRAP _ _) =>
-                (* we are an UNWRAP of a WRAP, so we can continue down the APPR *)
-                invoke_APPR' r et' out_evt
-                (* match et_size G et' with | errC e => err_failm (dispatch_error (Runtime e))
-                | resultC et'_size =>
-                  if (eqb (length rwev) et'_size)
-                  then (* we are the right inverse size! *)
-                    err_ret (evc rwev (asp_evt p ps et))
-                  else err_failm (dispatch_error (Runtime "UNWRAP of a WRAP ASP must have the same size of the WRAPed evidence"))
-                end *)
-              | Some (ev_arrow _ _ _) => err_failm (dispatch_error (Runtime "UNWRAP ASPs must be applied to a WRAP ASP"))
-              end
-            | _ => err_failm (dispatch_error (Runtime "UNWRAP ASPs must be applied to a WRAP ASP"))
-            end
-            *)
-          end
-
-        | EXTEND =>
-          match out_sig with
-          | OutUnwrap => err_failm (dispatch_error (Runtime "EXTEND ASPs must have OutN"))
-          | (OutN n) =>
-            (* first we split, left for the appr of extended part, right for rest *)
-            split_ev ;;
-            '(_, r_ev) <- (hoist_result (peel_n_rawev n r)) ;;
-
-            (* on left we do the dual of EXTEND *)
-            ev1 <- invoke_ASP (evc r out_evt) dual_par ;;
-
-            (* now on right, we work only on the remaining evidence *)
-            (* our new evidence is e' *)
-            (* now we do the recursive call *)
-            ev2 <- invoke_APPR' r_ev et' et' ;;
-            (* now join *)
-            join_seq ev1 ev2 
-          end
+    appr_asp_id <- get_asp_dual asp_id ;;
+    let dual_par := asp_paramsC appr_asp_id args targ_plc targ in
+    '(ev_arrow fwd in_sig out_sig) <- get_asp_type asp_id ;;
+    match fwd with
+    | REPLACE => (* Only do the dual ASP *)
+      invoke_ASP (evc r out_evt) dual_par
+    | WRAP =>
+      (* first do the dual ASP to unwrap *)
+      '(evc r'' et'') <- invoke_ASP (evc r out_evt) dual_par ;;
+      (* Check that the "UNWRAP" occured properly *)
+      match et_size G et'' with
+      | errC e => err_failm (dispatch_error (Runtime e))
+      | resultC n' => 
+        match et_size G et' with
+        | errC e => err_failm (dispatch_error (Runtime e))
+        | resultC n'' =>
+          if (eqb n' n'')
+          then (* The "UNWRAP" worked *)
+            (* so do the recursive call *)
+            invoke_APPR' r'' et' (asp_evt (session_plc sc) dual_par out_evt)
+          else err_failm (dispatch_error (Runtime err_str_appr_wrap_failed))
         end
+      end
+    | UNWRAP =>
+      (* to appraise an UNWRAP is to appraise whatever is below 
+      the UNWRAP and WRAP *)
+      match out_sig with
+      | OutN _ => err_failm (dispatch_error (Runtime err_str_unwrap_must_have_outwrap)) 
+      | OutUnwrap =>
+        e <- hoist_result (
+          apply_to_asp_under_wrap G asp_id (fun e => invoke_APPR' r e out_evt) et'
+        ) ;;
+        e
+      end
+
+    | EXTEND =>
+      match out_sig with
+      | OutUnwrap => err_failm (dispatch_error (Runtime err_str_extend_must_have_outn))
+      | (OutN n) =>
+        (* first we split, left for the appr of extended part, right for rest *)
+        split_ev ;;
+        '(_, r_ev) <- (hoist_result (peel_n_rawev n r)) ;;
+
+        (* on left we do the dual of EXTEND *)
+        ev1 <- invoke_ASP (evc r out_evt) dual_par ;;
+
+        (* now on right, we work only on the remaining evidence *)
+        (* our new evidence is e' *)
+        (* now we do the recursive call *)
+        ev2 <- invoke_APPR' r_ev et' et' ;;
+        (* now join *)
+        join_seq ev1 ev2 
       end
       (* ev' <- invoke_ASP (asp_paramsC appr_asp_id args targ_plc targ) ;;
       put_ev ev' *)
@@ -373,27 +292,13 @@ Fixpoint invoke_APPR' (r : RawEv) (et : EvidenceT) (out_evt : EvidenceT) {struct
           ev1 <- invoke_APPR' ev_l et1 (left_evt et1) ;;
           ev2 <- invoke_APPR' ev_r et2 (right_evt et2) ;;
           join_seq ev1 ev2
-        | _ => err_failm (dispatch_error (Runtime "Evidence splitting failed: rest of evidence not empty"))
+        | _ => err_failm (dispatch_error (Runtime err_str_ev_split_failed_not_empty))
         end
       (* ev1 <- invoke_APPR' r_ev et1 et1 ;;
       ev2 <- invoke_APPR' r_ev et2 et2 ;;
       join_seq ev1 ev2 *)
       end
     end
-    (* match out_evt with
-    | split_evt et1' et2' =>
-      if (eqb et1 et1')
-      then 
-        if (eqb et2 et2')
-        then 
-          '((evc r1' et1'), (evc r2' et2')) <- split_evidence (evc r et) et1 et2 ;;
-          ev1' <- invoke_APPR' r1' et1 et1' ;;
-          ev2' <- invoke_APPR' r2' et2 et2' ;;
-          join_seq ev1' ev2' 
-        else err_failm (dispatch_error (Runtime "Evidence splitting failed: et2 does not match"))
-      else err_failm (dispatch_error (Runtime "Evidence splitting failed: et1 does not match"))
-    | _ => err_failm (dispatch_error (Runtime "Evidence splitting failed: out_evt does not match"))
-    end *)
   end.
 
 Definition invoke_APPR (e : Evidence) : CVM Evidence :=
@@ -564,6 +469,8 @@ Ltac cvm_monad_unfold :=
   doRemote_session',
   check_cvm_policy,
   invoke_ASP,
+  get_asp_type,
+  get_asp_dual,
   bundle_asp,
   do_asp,
   clearEv,
