src/ErrorStringConstants.v
@@ -2,25 +2,13 @@
     Once instantiated, these should provide descriptive error messages for 
     dynamic error cases in Coq-extracted code. *)
 
-Require Import String.
+Require Import String Stringifiable.
+Require Import JSON_Type JSON_Admits.
+
 Open Scope string_scope.
 
-(* Global Context Errors *)
-Definition err_str_asp_no_type_sig := "ASP Type signature not found in the Global Context".
-
-Definition err_str_asp_no_compat_appr_asp := "Compatible Appraisal ASP not found in Global Context".
-
-
 (* AM and CVM Errors *)
-Definition empty_string := "empty_string".
-
-Definition errStr_amNonce := "errStr_amNonce".
-
-Definition errStr_peel_bs_am := "errStr_peel_bs_am".
-
-Definition errStr_peel_n_am := "errStr_peel_n_am".
-
-Definition errStr_requester_bound := "errStr_requester_bound".
+Definition errStr_peel_n_am := "Error peeling 'n' elements; ran out of RawEv".
 
 Definition errStr_disclosePolicy := "errStr_disclosePolicy".
 
@@ -63,6 +51,35 @@ Definition errStr_run_cvm_at_error_static := "errStr_run_cvm_at_error_static".
 
 Definition errStr_run_cvm_dispatch_unavailable := "errStr_run_cvm_dispatch_unavailable".
 
+(* Type/Size Errors *)
+Definition err_str_asp_bad_size `{Stringifiable nat} (got expect : nat) := 
+  "ASP requires input of size " ++ to_string expect ++ 
+  " but received input of size " ++ to_string got ++ "\n".
+
+(* Global Context Errors *)
+Definition err_str_asp_no_type_sig := 
+  "ASP Type signature not found in the Global Context".
+
+Definition err_str_asp_no_compat_appr_asp := 
+  "Compatible Appraisal ASP not found in Global Context".
+
+Definition err_str_asps_not_duals := "2 nested ASPs are not duals".
+
+Definition err_str_appr_asp_not_unwrap := "Compatible Appraisal ASP is not an UNWRAP ASP".
+
+Definition err_str_asp_is_not_wrap := "ASP is not a WRAP ASP".
+
+Definition err_str_no_possible_left_evt := ("No possible left_evt").
+Definition err_str_no_possible_right_evt := ("No possible right_evt").
+
+Definition err_str_asp_under_unwrap := "ASP under UNWRAP is not a WRAP".
+Definition err_str_wrap_asp_not_duals := "A WRAP and UNWRAP ASPs are not duals".
+Definition err_str_unwrap_only_asp := "UNWRAP ASPs must be applied to ASPs".
+Definition err_str_no_asp_under_evidence := "No ASP under evidence".
+Definition err_str_asp_at_bottom_not_wrap := "ASP at bottom of evidence is not a WRAP ASP".
+
+Definition err_str_cannot_have_outwrap := ("Invalid Output Signature of type 'OutUnwrap' on an ASP").
+
 (* JSON Converter Strings *)
 Definition errStr_json_to_manifest_set := "errStr_json_to_manifest_set".
 
@@ -76,19 +93,67 @@ Definition errStr_json_to_ASP_Locator := "errStr_json_to_ASP_Locator".
 
 Definition errStr_json_to_am_lib := "errStr_json_to_am_lib".
 
-Definition errStr_json_to_pair := "errStr_json_to_pair".
+Definition errStr_map_from_json := "errStr_map_from_json".
 
-Definition errStr_JSON_get_Object_key_not_found := "errStr_JSON_get_Object_key_not_found".
-Definition errStr_JSON_get_Object_not_a_json := "errStr_JSON_get_Object_not_a_json".
+Definition errStr_json_from_pair := "Error converting pair from JSON".
 
-Definition errStr_json_get_array_key_not_found := "errStr_json_get_array_key_not_found".
-Definition errStr_json_get_array_not_an_array := "errStr_json_get_array_not_an_array".
+Definition errStr_json_key_not_found (key : string) (js : JSON) := ("JSON: Key: '" ++ key ++ "' not found in JSON: '" ++ (JSON_to_string js) ++ "'").
 
-Definition errStr_json_get_string_key_not_found := "errStr_json_get_string_key_not_found".
-Definition errStr_json_get_string_not_a_string := "errStr_json_get_string_not_a_string".
+Definition errStr_json_wrong_type (key : string) (js : JSON) := ("JSON: Key: '" ++ key ++ "' had the wrong type in JSON: '" ++ (JSON_to_string js) ++ "'").
 
-Definition errStr_json_get_bool_key_not_found := "errStr_json_get_bool_key_not_found".
-Definition errStr_json_get_bool_not_a_bool := "errStr_json_get_bool_not_a_bool".
+Definition err_str_01 := "Invalid request type".
+
+Definition err_str_unwrap_must_have_outwrap := "UNWRAP ASPs must have an OutWrap output signature".
+
+Definition err_str_only_unwrap_can_be_outwrap := "Only UNWRAP ASPs can have an OutWrap output signature".
+
+Definition err_str_unwrap_of_wrap_same_size := "UNWRAP of a WRAP ASP must have the sime size as the WRAPed evidence".
+
+Definition err_str_unwrap_only_wrap := "UNWRAP ASPs must be appplied to a WRAP ASP".
+
+Definition err_str_appr_wrap_failed := "Appraisal for WRAP ASP failed. Size of input to wrap is not same as output of UNWRAP".
+
+Definition err_str_extend_must_have_outn := "EXTEND ASPs must have OutN".
+
+Definition err_str_ev_split_failed_not_empty := "Evidence splitting failed: rest of evidence not empty".
+
+Definition err_str_json_nat_string := "Error converting JSON to nat: JSON was not a string".
+
+Definition err_str_json_cannot_interp_nat := "Error:  cannot interpret nat string in Jsonifiable_nat".
+
+Definition err_str_json_parsing_outn := "Error parsing OutN from JSON (wrong number of arguments, expected 1)".
+
+Definition err_str_evoutsig_json_constructor := "Invalid EvOutSig JSON constructor name".
+
+Definition err_str_json_no_constructor_name_string := "JSON: No constructor name found in JSON".
+
+Definition err_str_invalid_evinsig_json := "Invalid EvInSig JSON".
+
+Definition err_str_json_parsing_failure_wrong_number_args :=
+  "Error parsing JSON: Wrong number of arguments".
+
+Definition err_str_json_invalid_constructor_name :=
+  "Error parsing JSON: Invalid constructor name".
+
+Definition err_str_json_parsing_SP := "Error parsing SP from JSON (not ALL or NONE)".
+
+Definition err_str_json_parsing_ASPC := "Error parsing ASPC from JSON".
+
+Definition err_str_invalid_evidence_json := "Invalid Evidence JSON".
+
+Definition err_str_parsing_global_ctx := "Error parsing Global Context from JSON".
+
+Definition err_str_json_unrecognized_constructor := "Unrecognized constructor in JSON".
+
+Definition err_str_list_json_to_manifest_set := "Error converting list from JSON to Manifest Set".
+
+Definition err_str_appr_compute_evt_neq := "Error in appraisal procedure computation, type of evidence passed into an appraisal procedure does not match the expected type (evidence types are not equivalent)"%string. 
+Definition err_str_appr_compute_appr_wrap_no_unwrap := "Error in appraisal procedure computation: Attempting to appraise WRAPPED evidence but the dual appraisal ASP is not an UNWRAP."%string.
+Definition err_str_appr_not_originally_a_wrap := "Error in appraisal procedure computation: Attempting to appraise UNWRAPPED evidence but the UNWRAPPED evidence was not originally a WRAP."%string.
+Definition err_str_appr_only_allow_on_asp := "Error in appraisal procedure computation: Attempting to appraise UNWRAPPED evidence but evidence that was UNWRAPPED was not an ASP (UNWRAP can only be applied to an ASP input)."%string.
+
+Definition err_str_split_evidence_not_split := "Error in appraisal procedure computation, type of evidence passed into a split appraisal procedure is not a split evidence type"%string.
+
 
 Close Scope string_scope.
 
