src/Interface_Strings_Vars.v
@@ -26,3 +26,8 @@ Definition STR_ASP_ID : string := "ASP_ID".
 Definition STR_ASP_ARGS : string := "ASP_ARGS".
 Definition STR_ASP_PLC : string := "ASP_PLC".
 Definition STR_ASP_TARG_ID : string := "ASP_TARG_ID".
+
+Definition STR_Session_Plc : string := "Session_Plc".
+Definition STR_Plc_Mapping : string := "Plc_Mapping".
+Definition STR_PubKey_Mapping : string := "PubKey_Mapping".
+Definition STR_Session_Context : string := "Session_Context".
