src/AM_Json_Interfaces.v
@@ -27,5 +27,5 @@ Definition handle_AM_request_JSON (conf : AM_Manager_Config) (js : JSON) (nonceV
       (* TODO: Fill this in when negotiation is implemented *)
       ErrorResponseJSON errStr_negotiation_not_implemented
     )
-    else ErrorResponseJSON "Invalid request type"
+    else ErrorResponseJSON err_str_01
   end.
