src/JSON_Core_Strings.v
@@ -1,0 +1,55 @@
+Require Import String.
+
+Definition type_string_constant : string := "CONSTRUCTOR".
+Definition body_string_constant : string := "BODY".
+Definition type_sep : string := "_".
+
+Definition fwd_name_constant  : string := "FWD".
+Definition replace_name_constant : string := "REPLACE".
+Definition wrap_name_constant : string := "WRAP".
+Definition unwrap_name_constant : string := "UNWRAP".
+Definition extend_name_constant : string := "EXTEND".
+
+Definition mt_name_constant : string := "mt_evt".
+Definition nonce_evt_name_constant : string := "nonce_evt".
+Definition asp_evt_name_constant : string := "asp_evt".
+Definition left_evt_name_constant : string := "left_evt".
+Definition right_evt_name_constant : string := "right_evt".
+
+Definition split_evt_name_constant : string := "split_evt".
+
+Definition asp_name_constant  : string := "asp".
+Definition null_name_constant : string := "NULL".
+Definition appr_name_constant : string := "APPR".
+Definition copy_name_constant : string := "CPY".
+Definition aspc_name_constant : string := "ASPC".
+Definition sig_name_constant  : string := "SIG".
+Definition hsh_name_constant  : string := "HSH".
+Definition enc_name_constant  : string := "ENC".
+
+Definition evidencet_name_constant : string := "EvidenceT".
+
+Definition att_name_constant  : string := "att".
+Definition lseq_name_constant : string := "lseq".
+Definition bseq_name_constant : string := "bseq".
+Definition bpar_name_constant : string := "bpar".
+
+Definition rawev_name_constant : string := "RawEv".
+
+Definition sp_name_constant   : string := "SP".
+Definition all_name_constant  : string := "ALL".
+Definition none_name_constant : string := "NONE".
+
+Definition split1_name_constant : string := "split1".
+Definition split2_name_constant : string := "split2".
+
+Definition ev_out_sig_name_constant : string := "EvOutSig".
+Definition outn_name_constant : string := "OutN".
+Definition outunwrap_name_constant : string := "OutUnwrap".
+
+Definition asp_types_name_constant : string := "ASP_Types".
+Definition asp_comps_name_constant : string := "ASP_Comps".
+
+Definition ev_in_sig_name_constant : string := "EvInSig".
+
+Definition term_plc_list_name_constant : string := "Term_Plc_List".
